src/wps.v
@@ -298,13 +298,6 @@ Lemma wps_confront_Stackable l r t (A:Type) (EA:Enc A) (Q:A -> iProp Σ) :
   wps (Some r) t Q.
 Proof. apply wpc_confront_Stackable. Qed.
 
-Lemma wps_confront_vmapsfrom v1 v2 q1 q2 ls1 ls2 r t (A:Type) (EA:Enc A) (Q:A -> iProp Σ) :
-  (is_loc v1 -> is_loc v2 -> 1 < q1 + q2)%Qz ->
-  v1 ↤?{q1} ls1 ∗ v2 ↤?{q2} ls2 -∗
-  (v1 ↤?{q1} ls1 ∗ v2 ↤?{q2} ls2 ∗ ⌜diff_loc v1 v2⌝  -∗ wps (Some r) t Q) -∗
-  wps (Some r) t Q.
-Proof. apply wpc_confront_vmapsfrom. Qed.
-
 Lemma wps_cleanup_vsingleton l' v q ls X t (A:Type) (EA:Enc A) (Q:A -> iProp Σ) :
   v ↤?{q} ls ∗ †l' -∗
   (v ↤?{q} (ls ⊎ {[-l'-]}) ∗ †l' -∗ wps X t Q) -∗
